src/impl/TLS13.Impl.Server.fsti
@@ -11,6 +11,7 @@ module CM = TLS13.Impl.ConnectionState.Model
 module CR = TLS13.Impl.ConnectionState.Repr
 module CQ = TLS13.Impl.ConnectionState.Queries
 module ST = TLS13.Impl.Server.Types
+module Seq = FStar.Seq
 module SZ = FStar.SizeT
 module U8 = FStar.UInt8
 
@@ -63,7 +64,7 @@ fn new_server
                   (CR.server_initial_state
                     (Ghost.reveal 'certificate_chain_bytes)
                     (Ghost.reveal 'credential_identity_bytes)) /\
-                CS.connection_state_raw_to_message_replay_consistent
+                ST.server_raw_to_message_replay_consistent
                   (CR.server_initial_state
                     (Ghost.reveal 'certificate_chain_bytes)
                     (Ghost.reveal 'credential_identity_bytes)) /\
@@ -71,15 +72,7 @@ fn new_server
                   (CR.server_initial_state
                     (Ghost.reveal 'certificate_chain_bytes)
                     (Ghost.reveal 'credential_identity_bytes)) /\
-                CS.connection_state_sent_seal_key_schedule_replay_consistent
-                  (CR.server_initial_state
-                    (Ghost.reveal 'certificate_chain_bytes)
-                    (Ghost.reveal 'credential_identity_bytes)) /\
                 CS.connection_state_received_decode_replay_consistent
-                  (CR.server_initial_state
-                    (Ghost.reveal 'certificate_chain_bytes)
-                    (Ghost.reveal 'credential_identity_bytes)) /\
-                CS.connection_state_received_decode_key_schedule_replay_consistent
                   (CR.server_initial_state
                     (Ghost.reveal 'certificate_chain_bytes)
                     (Ghost.reveal 'credential_identity_bytes)) /\
@@ -96,3 +89,40 @@ fn next_local_action
   ensures connection_exactly s 'st0 **
           pure (ST.server_state_correct 'st0 /\
                 next_local_action_sound 'st0 action)
+
+fn process_local_event
+  (s:server)
+  (kind:ST.local_event_kind)
+  (payload:array U8.t)
+  (payload_len:SZ.t)
+  (network_out:array U8.t)
+  (network_out_len:SZ.t)
+  (app_out:array U8.t)
+  (app_out_len:SZ.t)
+  requires connection_exactly s 'st0 **
+           pts_to payload 'payload_bytes **
+           pts_to network_out 'old_network_out **
+           pts_to app_out 'old_app_out **
+           pure (B.length 'payload_bytes == SZ.v payload_len /\
+                 B.length 'old_network_out == SZ.v network_out_len /\
+                 B.length 'old_app_out == SZ.v app_out_len /\
+                 ST.server_end_to_end_invariant 'st0 /\
+                 kind == ST.LocalStartServer /\
+                 Seq.equal (Ghost.reveal 'payload_bytes) B.empty /\
+                 CM.can_start_server 'st0)
+  returns resp:ST.server_response
+  ensures exists* st1 network_out_bytes app_out_bytes.
+          connection_exactly s st1 **
+          pts_to payload 'payload_bytes **
+          pts_to network_out network_out_bytes **
+          pts_to app_out app_out_bytes **
+          pure (B.length network_out_bytes == SZ.v network_out_len /\
+                B.length app_out_bytes == SZ.v app_out_len /\
+                ST.server_local_event_end_to_end_correct
+                  'st0
+                  st1
+                  resp
+                  kind
+                  (Ghost.reveal 'payload_bytes)
+                  network_out_bytes
+                  app_out_bytes)
